Introduce sig^+ Notation to replace the sig' Definition

TM/Code/CodeTM.v
@@ -68,6 +68,8 @@ Proof. destruct t; cbn; reflexivity. Qed.
 Hint Rewrite mapTape_local : tape.
 
 
+Notation "sig '^+'" := (FinType(EqType(sig + bool))) (at level 0) : type_scope.
+
 Section Fix_Sig.
   
   Variable (sig : finType).
@@ -78,28 +80,31 @@ Section Fix_Sig.
     Variable (X : Type) (cX : codeable sig X).
 
     (* Extend sig with a start end a end symbol *)
-    Definition sig' : finType := FinType(EqType((sig + bool))) % type.
+
+    Check sig^+.
+    Check tapes sig^+ 42.
+    Check (sig + bool) % type.
 
     Definition START : bool := false.
     Definition STOP  : bool := true.
 
-    Instance codeX : codeable sig' X := Encode_Map cX          (@retract_inl sig bool).
-    Instance codeS : codeable sig' bool := Encode_Map Encode_Bool (@retract_inr sig bool).
+    Instance codeX : codeable sig^+ X := Encode_Map cX          (@retract_inl sig bool).
+    Instance codeS : codeable sig^+ bool := Encode_Map Encode_Bool (@retract_inr sig bool).
 
-    Definition tape_encodes_r (t : tape sig') (x : X) (r1 r2 : list sig') :=
+    Definition tape_encodes_r (t : tape sig^+) (x : X) (r1 r2 : list sig^+) :=
       left t = encode START ++ r1 /\ tape_local t = encode x ++ encode STOP ++ r2.
 
-    Definition tape_encodes (t : tape sig') (x : X) : Prop :=
-      exists r1 r2 : list sig', tape_encodes_r t x r1 r2.
+    Definition tape_encodes (t : tape sig^+) (x : X) : Prop :=
+      exists r1 r2 : list sig^+, tape_encodes_r t x r1 r2.
 
-    Lemma tape_encodes_r_injective (t : tape sig') (x1 x2 : X) (r1 r2 s1 s2 : list sig') :
+    Lemma tape_encodes_r_injective (t : tape sig^+) (x1 x2 : X) (r1 r2 s1 s2 : list sig^+) :
       tape_encodes_r t x1 r1 r2 -> tape_encodes_r t x2 s1 s2 -> x1 = x2 /\ r1 = s1 /\ r2 = s2.
     Proof.
       intros (H2&H2') (H1&H1'). rewrite H2 in H1; clear H2. rewrite H2' in H1'. clear H2'. cbn in *.
       eapply encode_map_injective in H1' as (->&H2). inv H1. inv H2. tauto. eapply retract_inl.
     Qed.
 
-    Lemma tape_encodes_injective (t : tape sig') (x1 x2 : X) :
+    Lemma tape_encodes_injective (t : tape sig^+) (x1 x2 : X) :
       tape_encodes t x1 -> tape_encodes t x2 -> x1 = x2.
     Proof.
       intros (r1&r2&H2) (s1&s2&H1). eapply tape_encodes_r_injective; eauto.
@@ -114,13 +119,13 @@ Section Fix_Sig.
     Variable (X Y : Type) (cX : codeable sig X) (cY : codeable sig Y).
     Variable F : finType.
 
-    Definition Computes (f : X -> Y) : relation (tapes sig' n_tapes) :=
+    Definition Computes (f : X -> Y) : relation (tapes (sig ^+) n_tapes) :=
       fun tin tout =>
         forall (x : X),
           tape_encodes _ ( tin[@i]) x ->
           tape_encodes _ (tout[@j]) (f x).
 
-    Definition Computes_Rel (f : X -> Y) : Rel (tapes sig' n_tapes) (F * tapes sig' n_tapes) :=
+    Definition Computes_Rel (f : X -> Y) : Rel (tapes sig^+ n_tapes) (F * tapes sig^+ n_tapes) :=
       ignoreParam (Computes f).
 
     Section Computes_Ext.
@@ -136,7 +141,7 @@ Section Fix_Sig.
         - intros t t' H1. hnf in *. intros x. specialize (H1 x). rewrite (ext x). eauto.
       Qed.
 
-      Variable pM : { M : mTM sig' n_tapes & states M -> F }.
+      Variable pM : { M : mTM sig^+ n_tapes & states M -> F }.
 
       Lemma Computes_Ext_WRealise :
         pM ⊫ Computes_Rel f' ->
@@ -169,15 +174,14 @@ Section Fix_Sig.
     End Computes_Ext.
   End Computes.
 
-
   Section Computes_Composes.
     Variable (X Y Z : Type) (cX : codeable sig X) (cY : codeable sig Y) (cZ : codeable sig Z).
     Variable (f : X -> Y) (g : Y -> Z).
     Variable (n_tapes : nat).
     Variable (i1 i2 i3 : Fin.t n_tapes).
     Variable (F1 F2 : finType).
-    Variable (pM : {M : mTM sig' n_tapes & states M -> F1}).
-    Variable (pN : {N : mTM sig' n_tapes & states N -> F2}).
+    Variable (pM : {M : mTM sig^+ n_tapes & states M -> F1}).
+    Variable (pN : {N : mTM sig^+ n_tapes & states N -> F2}).
 
     Lemma compose_Computes_Realise (iin iout : Fin.t n_tapes) :
       pM ⊨ Computes_Rel (F := F1) i1 i2 _ _ f ->
@@ -220,14 +224,14 @@ Section Fix_Sig.
     Variable f : X -> Y -> Z.
     Variable F : finType.
 
-    Definition Computes2 : relation (tapes sig' n_tapes) :=
+    Definition Computes2 : relation (tapes sig^+ n_tapes) :=
       fun tin tout =>
         forall (x : X) (y : Y),
           tape_encodes _ ( tin[@i]) x ->
           tape_encodes _ ( tin[@j]) y ->
           tape_encodes _ (tout[@k]) (f x y).
 
-    Definition Computes2_Rel : Rel (tapes sig' n_tapes) (F * tapes sig' n_tapes) :=
+    Definition Computes2_Rel : Rel (tapes sig^+ n_tapes) (F * tapes sig^+ n_tapes) :=
       ignoreParam (Computes2).
 
   End Computes2.
